### Definition of the Tangent Plane
Suppose a surface $S$ has equation $z=f(x,y)$, where $f$ has continuous first partial derivatives. 
Suppose we also have a point $P(x_0,y_0,z_0)$ which lies on $S$. Let $C_1$ and $C_2$ be the curves gained from intersecting the vertical planes $x=x_0$ and $y=y_0$, and $T_1$ and $T_2$ be the tangent lines to curves $C_1$ and $C_2$. 
Given this, the **tangent plane** will contain both of the tangent lines $T_1$ and $T_2$. 

Recall the equation of a plane is: $$A(x-x_{0})+B(y-y_{0})+C(z-z_{0})=0$$
If we put the equation in terms of the x and y axis to get the z, we would get$$-\frac{A}{C}(x-x_{0})-\frac{B}{C}(y-y_{0})=z-z_{0}$$
Let this be the equation of the tangent plane $P$. Given $p$ is the tangent plane, its intersection with the plane $y=y_0$ must be one of the tangent lines, given $P$ has every line tangent to the plane. We'll refer to this line as $T_1$.
We can find $T_1$ by plugging in $y=y_0$:$$-\frac{A}{C}(x-x_{0})=z-z_{0}$$
By setting $a=-\frac{A}{C}$, we can rewrite this as
$$a(x-x_0)=z-z_0$$
	This is the point slope form of the equation of a line.
	$a$ appears to be the slope, and we know the slope of the tangent line at point $P$ is the partial derivative at $P$. 
	$$f_{x}(x_{0},y_{0})(x-x_{0})+z_{0}=z$$
We can use a similar principle for the y-axis.
$$b=-\frac{B}{C}$$
$$b(y-y_{0})+z_{0}=z$$
	$$f_{y}(y_{0},y_{0})(y-y_{0})+z_{0}=z$$This equation will represent tangent line $T_2$.
Plugging in our values for $a$ and $b$ into the plane equation, we find
$$\boxed{f_{x}(x_{0},y_{0})(x-x_{0})+f_{y}(x_{0},y_{0})(y-y_{0})=z-z_{0}}$$
This is the equation for a tangent plane to a surface $S$, where $z_0$ is $f(x_{0},y_{0})$