### The Chain Rule - Case 1
Imagine we have a function $z=f(x,y)$ where $x=r(t)$ and $y=s(t)$.  Then,$$\frac{\partial z}{\partial t}=\frac{\partial f}{\partial x}\frac{dx}{dt}+\frac{\partial f}{\partial y}\frac{dy}{dt} $$Example: Find $\frac{\partial z}{\partial t}$ of $z=xy^3-x^2y$, where $x=t^2 +1$ and $y=t^2-1$
$$\frac{\partial z}{\partial t}=(y^3+2xy)(2t)+(3xy^2-x^2)(2t)$$
$$\frac{\partial z}{\partial t}=((t^2-1)^3+2(t^2+1)(t^2-1))(2t)+(3(t^2+1)(t^2-1)^2-(t^2+1)^2)(2t)$$
$$\frac{\partial z}{\partial t}=((t^2-1)^3+2(t^4-1))(2t)+(3(t^2+1)(t^2-1)^2-(t^2+1)^2)(2t)$$
ehhh i dont feel like doing the rest of this LOL


### The Chain Rule - Case 2
Imagine we have another function $z=f(x,y)$ where $x=g(s,t)$ and $y=h(s,t)$. 
We can get the derivative in terms of both $s$ and $t$.
$$\frac{\partial z}{\partial t}=\frac{\partial f}{\partial x}\frac{\partial x}{\partial t}+\frac{\partial z}{\partial y}\frac{\partial y}{\partial t}$$
$$\frac{\partial z}{\partial s}=\frac{\partial f}{\partial x}\frac{\partial x}{\partial s}+\frac{\partial z}{\partial y}\frac{\partial y}{\partial s}$$
The process is identical except you must use partial derivatives.
Example: $z=\arctan(x^2+y^2), x = s\ln(t),y=te^s$, find $\frac{\partial d}{\partial t}$
$$\frac{\partial d}{\partial t}=\frac{\partial z}{\partial x}\frac{\partial x}{\partial t}+\frac{\partial z}{\partial y}\frac{\partial y}{\partial t}$$
$$\frac{\partial d}{\partial t}=\frac{2xs}{t((x^2+y^2)^2+1) }+\frac{2ye^s}{1+(x^2+y^2)^2}$$
### The Chain Rule - General Case

We may also have a circumstance where we have a function $w=f(x,y,z)$, where $x=r(u,v)$, $y=s(u,v)$, and $z=t(u,v)$, and we need to find $\frac{\partial w}{\partial u}$ or  $\frac{\partial w}{\partial v}$. 
$$\frac{\partial w}{\partial u}=\frac{\partial w}{\partial x}\frac{\partial x}{\partial u}+\frac{\partial w}{\partial y}\frac{\partial y}{\partial u}+\frac{\partial w}{\partial z}\frac{\partial z}{\partial u}$$

Generally, for a function $w$ of $n$ variables, differentiating it with respect to a variable $u$ means you must first take the partial derivative of $w$ with respect to each variable and multiply each with the partial derivative of each variable with respect to $u$.
### Higher-order derivatives
Given a function $z=x^3-y^3$ where $x=(u^2+1)v^2$, and $y=u^3(v+1)$,  find $\frac{\partial^2 z}{\partial u^2}$.

First, we must find $\frac{\partial d}{\partial u}$.
$$\frac{\partial z}{\partial u}=\frac{\partial z}{\partial x}\frac{\partial x}{\partial u}+\frac{\partial z}{\partial y}\frac{\partial y}{\partial u}$$
$$
\frac{\partial z}{\partial u}=(3x^2-y^3)(2v^2u)+(x^3-3y^2)(3vu^2+3u^2)
$$


### Implicit Differentiation
Implicit differentiation is done through the Chain Rule in multivariable calculus.
Suppose we have an equation $F(x,y)=0$, which will define $y$ implicitly as a differentiable function of $x$ ($y=f(x)$). Let's also suppose that $F(x,f(x))=0$ for all $x$ in the domain of $F$. If $F$ is differentiable, we can apply case 1 of the Chain Rule to differentiate both sides of the equation $F(x,y)=0$ with respect to $x$.
$$\frac{\partial F}{\partial x}\frac{\partial x}{\partial x}+\frac{\partial F}{\partial y}\frac{dy}{dx}=0$$
We can simplify (dx/dx = 1)
$$\frac{\partial F}{\partial x}+\frac{\partial F}{\partial y}\frac{dy}{d x}=0$$To obtain the implicit differentiation of $y$ with respect to $x$, we can solve for $\frac{\partial y}{\partial x}$ in this equation
$$-\frac{\frac{\partial F}{\partial y}}{\frac{\partial F}{\partial x}}=\frac{dy}{dx}$$
$$\boxed{-\frac{F_{y}}{F_{x}}=\frac{dy}{dx}}$$
Example: find $\frac{dy}{dx}$ if $x^3+y^3=6xy$.
First, the expression must be equal to 0. $$x^3+y^3-6xy=0$$
Now we can perform implicit differentiation.
$$\frac{dy}{dx}=\frac{3y^2-6x}{3x^2-6y}$$
$$\boxed{\frac{dy}{dx}=\frac{y^2-2x}{x^2-2y}}$$
#### The Implicit Function Theorem
- If a function $F$ is defined on a disk containing  $(a,b)$ where $F(a,b)=0$,$F_{y}(a,b)\not=0$, and $F_x$ and $F_y$ are continuous on the disk, then the equation $F(x,y)=0$ defines $y$ as a function of $x$ near the point $(a,b)$ and the derivative of this function is given by the above equation.
	Example: Implicit differentiation in 3 variables:
	Suppose $z$ is a function $z=f(x,y)$ and is given implicitly as $F(x,y,z)=0$. This means $F(x,y,f(x,y))=0$ (assuming all conditions of the implicit function theorem are met). Given this, we can take the derivative of both sides of the equation using the Chain Rule. $$\frac{\partial F}{\partial x} \frac{\partial x}{\partial x} + \frac{\partial F}{\partial y} \frac{\partial y}{\partial x}+ \frac{\partial F}{\partial z} \frac{\partial z}{\partial x}=0$$
	We can simplify ($\frac{\partial x}{\partial x}=1$,$\frac{\partial y}{\partial x}=0$) to make$$\frac{\partial F}{\partial x}+ \frac{\partial F}{\partial z} \frac{\partial z}{\partial x}=0$$ Solving for $\frac{\partial z}{\partial x}$:
	$$$$